Typing rules for global set/get; clean up

theories/typing.v
@@ -7,36 +7,46 @@ Require Import RecordUpdate.RecordUpdate.
 
 Require Import RichWasm.syntax.
 
-Definition local_context := list type.
+Record module_ctx :=
+  { mc_globals : list global_type }.
 
-Record function_context :=
+Definition local_ctx := list type.
+
+Record function_ctx :=
   { fc_result_type : list type;
-    fc_labels : list (list type * local_context);
+    fc_labels : list (list type * local_ctx);
     fc_location_vars : nat;
     fc_rep_vars : nat;
     fc_type_vars : list kind }.
 
-Global Instance eta_function_context : Settable _ :=
-  settable! Build_function_context
+Definition fc_empty : function_ctx :=
+  {| fc_result_type := [];
+     fc_labels := [];
+     fc_location_vars := 0;
+     fc_rep_vars := 0;
+     fc_type_vars := [] |}.
+
+Global Instance eta_function_ctx : Settable _ :=
+  settable! Build_function_ctx
   <fc_result_type; fc_labels; fc_location_vars; fc_rep_vars; fc_type_vars>.
 
-Definition update_locals (le : local_effect) (L : local_context) : local_context :=
+Definition update_locals (le : local_effect) (L : local_ctx) : local_ctx :=
   fold_left (fun acc '(i, τ) => <[ i := τ ]> acc) le L.
 
-Inductive rep_ok : function_context -> representation -> Prop :=
-| VarR_OK (F : function_context) (ϱ : variable) :
+Inductive rep_ok : function_ctx -> representation -> Prop :=
+| VarR_OK (F : function_ctx) (ϱ : variable) :
   ϱ < F.(fc_rep_vars) -> rep_ok F (VarR ϱ)
-| SumR_OK (F : function_context) (rs : list representation) :
+| SumR_OK (F : function_ctx) (rs : list representation) :
   Forall (rep_ok F) rs -> rep_ok F (SumR rs)
-| ProdR_OK (F : function_context) (rs : list representation) :
+| ProdR_OK (F : function_ctx) (rs : list representation) :
   Forall (rep_ok F) rs -> rep_ok F (ProdR rs)
-| PrimR_OK (F : function_context) (p : primitive_rep) :
+| PrimR_OK (F : function_ctx) (p : primitive_rep) :
   rep_ok F (PrimR p)
-| DynR_OK (F : function_context) :
+| DynR_OK (F : function_ctx) :
   rep_ok F DynR.
 
-Inductive kind_ok : function_context -> kind -> Prop :=
-| TYPE_OK (F : function_context) (r : representation) (l : linearity) (h : heapability) :
+Inductive kind_ok : function_ctx -> kind -> Prop :=
+| TYPE_OK (F : function_ctx) (r : representation) (l : linearity) (h : heapability) :
   rep_ok F r -> kind_ok F (TYPE r l h).
 
 Inductive has_mono_size : representation -> nat -> Prop :=
@@ -58,166 +68,161 @@ Inductive has_mono_size : representation -> nat -> Prop :=
 | SizeF64R :
   has_mono_size (PrimR F64R) 2.
 
-Inductive has_kind : function_context -> type -> kind -> Prop :=
-| KSubLin (F : function_context) (τ : type) (r : representation) (h : heapability) :
+Inductive has_kind : function_ctx -> type -> kind -> Prop :=
+| KSubLin (F : function_ctx) (τ : type) (r : representation) (h : heapability) :
   has_kind F τ (TYPE r Unr h) ->
   has_kind F τ (TYPE r Lin h)
-| KSubHeap (F : function_context) (τ : type) (r : representation) (l : linearity) :
+| KSubHeap (F : function_ctx) (τ : type) (r : representation) (l : linearity) :
   has_kind F τ (TYPE r l Heapable) ->
   has_kind F τ (TYPE r l Unheapable)
-| KVar (F : function_context) (α : variable) (κ : kind) :
+| KVar (F : function_ctx) (α : variable) (κ : kind) :
   F.(fc_type_vars) !! α = Some κ ->
   kind_ok F κ ->
   has_kind F (VarT α) κ
-| KI32 (F : function_context) :
+| KI32 (F : function_ctx) :
   has_kind F (NumT (IntT I32T)) (TYPE (PrimR I32R) Unr Heapable)
-| KI64 (F : function_context) :
+| KI64 (F : function_ctx) :
   has_kind F (NumT (IntT I64T)) (TYPE (PrimR I64R) Unr Heapable)
-| KF32 (F : function_context) :
+| KF32 (F : function_ctx) :
   has_kind F (NumT (FloatT F32T)) (TYPE (PrimR F32R) Unr Heapable)
-| KF64 (F : function_context) :
+| KF64 (F : function_ctx) :
   has_kind F (NumT (FloatT F64T)) (TYPE (PrimR F64R) Unr Heapable)
 | KSum
-    (F : function_context) (τs : list type) (rs : list representation) (l : linearity)
+    (F : function_ctx) (τs : list type) (rs : list representation) (l : linearity)
     (h : heapability) :
   Forall2 (fun τ r => has_kind F τ (TYPE r l h)) τs rs ->
   has_kind F (SumT τs) (TYPE (SumR rs) l h)
 | KProd
-    (F : function_context) (τs : list type) (rs : list representation) (l : linearity)
+    (F : function_ctx) (τs : list type) (rs : list representation) (l : linearity)
     (h : heapability) :
   Forall2 (fun τ r => has_kind F τ (TYPE r l h)) τs rs ->
   has_kind F (ProdT τs) (TYPE (ProdR rs) l h)
-| KArray (F : function_context) (τ : type) (r : representation) :
+| KArray (F : function_ctx) (τ : type) (r : representation) :
   has_kind F τ (TYPE r Unr Heapable) ->
   has_kind F (ArrayT τ) (TYPE DynR Unr Heapable)
-| KExLoc (F : function_context) (τ : type) (κ : kind) :
+| KExLoc (F : function_ctx) (τ : type) (κ : kind) :
   has_kind (set fc_location_vars S F) τ κ ->
   has_kind F (ExT ELoc τ) κ
-| KExType (F : function_context) (τ : type) (κ0 κ : kind) :
+| KExType (F : function_ctx) (τ : type) (κ0 κ : kind) :
   has_kind (set fc_type_vars (cons κ0) F) τ κ ->
   has_kind F (ExT (EType κ0) τ) κ
-| KRec (F : function_context) (τ : type) (κ : kind) :
+| KRec (F : function_ctx) (τ : type) (κ : kind) :
   (* TODO: Unfold. *)
   has_kind F τ κ ->
   has_kind F (RecT τ) κ
-| KPtr (F : function_context) (ℓ : location) :
+| KPtr (F : function_ctx) (ℓ : location) :
   has_kind F (PtrT ℓ) (TYPE (PrimR PtrR) Unr Heapable)
-| KCap (F : function_context) (ℓ : location) (τ : type) :
+| KCap (F : function_ctx) (ℓ : location) (τ : type) :
   has_kind F (CapT ℓ τ) (TYPE (ProdR []) Lin Unheapable)
-| KBoxUniq (F : function_context) (ℓ : location) (τ : type) :
+| KBoxUniq (F : function_ctx) (ℓ : location) (τ : type) :
   has_kind F (BoxT OwnUniq ℓ τ) (TYPE (PrimR PtrR) Lin Heapable)
-| KBoxGC (F : function_context) (ℓ : location) (τ : type) :
+| KBoxGC (F : function_ctx) (ℓ : location) (τ : type) :
   has_kind F (BoxT OwnGC ℓ τ) (TYPE (PrimR PtrR) Unr Heapable)
-| KCoderef (F : function_context) (χ : function_type) :
+| KCoderef (F : function_ctx) (χ : function_type) :
   has_kind F (CoderefT χ) (TYPE (PrimR I32R) Unr Heapable)
 | KRepT
-    (F : function_context) (r0 r : representation) (sz0 sz : nat) (τ : type) (l : linearity)
+    (F : function_ctx) (r0 r : representation) (sz0 sz : nat) (τ : type) (l : linearity)
     (h : heapability) :
   sz0 <= sz ->
   has_mono_size r0 sz0 ->
   has_mono_size r sz ->
   has_kind F τ (TYPE r0 l h) ->
   has_kind F (RepT r τ) (TYPE r l h)
-| KSize (F : function_context) (r : representation) :
+| KSize (F : function_ctx) (r : representation) :
   has_kind F (SizeT r) (TYPE (PrimR I32R) Unr Heapable).
 
-Inductive has_rep : function_context -> type -> representation -> Prop :=
-| RepTYPE (F : function_context) (τ : type) (r : representation) (l : linearity) (h : heapability) :
+Inductive has_rep : function_ctx -> type -> representation -> Prop :=
+| RepTYPE (F : function_ctx) (τ : type) (r : representation) (l : linearity) (h : heapability) :
   has_kind F τ (TYPE r l h) ->
   has_rep F τ r.
 
-Inductive is_unrestricted : function_context -> type -> Prop :=
-| UnrTYPE (F : function_context) (τ : type) (r : representation) (h : heapability) :
+Inductive is_unrestricted : function_ctx -> type -> Prop :=
+| UnrTYPE (F : function_ctx) (τ : type) (r : representation) (h : heapability) :
   has_kind F τ (TYPE r Unr h) ->
   is_unrestricted F τ.
+
+Inductive module_ctx_ok : module_ctx -> Prop :=
+| MC_OK (τgs : list global_type) :
+  Forall (fun '(GlobalT _ τ) => is_unrestricted fc_empty τ) τgs ->
+  module_ctx_ok {| mc_globals := τgs |}.
 
 (* TODO *)
 Inductive num_instr_has_type : num_instr -> arrow_type -> Prop :=.
 
 Inductive instr_has_type {A : Type} :
-  function_context -> local_context -> instr A -> arrow_type -> local_context -> Prop :=
-| TNop (F : function_context) (L : local_context) (ann : A) :
-  instr_has_type F L (INop ann) (ArrowT [] []) L
-| TDrop (F : function_context) (L : local_context) (ann : A) (τ : type) :
+  module_ctx -> function_ctx -> local_ctx -> instr A -> arrow_type -> local_ctx -> Prop :=
+| TNop M F L ann :
+  instr_has_type M F L (INop ann) (ArrowT [] []) L
+| TDrop M F L ann τ :
   is_unrestricted F τ ->
-  instr_has_type F L (IDrop ann) (ArrowT [τ] []) L
-| TUnreachable
-    (F : function_context) (L L' : local_context) (ann : A) (τs1 τs2 : list type) (le : local_effect) :
+  instr_has_type M F L (IDrop ann) (ArrowT [τ] []) L
+| TUnreachable M F L L' ann τs1 τs2 le :
   L' = update_locals le L ->
-  instr_has_type F L (IUnreachable ann) (ArrowT τs1 τs2) L
-| TNum (F : function_context) (L : local_context) (ann : A) (en : num_instr) (τa : arrow_type) :
+  instr_has_type M F L (IUnreachable ann) (ArrowT τs1 τs2) L
+| TNum M F L ann en τa :
   num_instr_has_type en τa ->
-  instr_has_type F L (INum ann en) τa L
-| TNumConst (F : function_context) (L : local_context) (ann : A) (τn : num_type) (n : nat) :
-  instr_has_type F L (INumConst ann τn n) (ArrowT [] [NumT τn]) L
-| TBlock
-    (F F' : function_context) (L L' : local_context) (ann : A) (τs1 τs2 : list type)
-    (le : local_effect) (es : expr A) :
+  instr_has_type M F L (INum ann en) τa L
+| TNumConst M F L ann τn n :
+  instr_has_type M F L (INumConst ann τn n) (ArrowT [] [NumT τn]) L
+| TBlock M F F' L L' ann τs1 τs2 le es :
   F' = set fc_labels (cons (τs2, L')) F ->
   L' = update_locals le L ->
-  expr_has_type F L es (ArrowT τs1 τs2) L' ->
-  instr_has_type F L (IBlock ann (ArrowT τs1 τs2) le es) (ArrowT τs1 τs2) L'
-| TLoop
-    (F F' : function_context) (L : local_context) (ann : A) (τs1 τs2 : list type) (es : expr A) :
+  expr_has_type M F L es (ArrowT τs1 τs2) L' ->
+  instr_has_type M F L (IBlock ann (ArrowT τs1 τs2) le es) (ArrowT τs1 τs2) L'
+| TLoop M F F' L ann τs1 τs2 es :
   F' = set fc_labels (cons (τs1, L)) F ->
-  expr_has_type F L es (ArrowT τs1 τs2) L ->
-  instr_has_type F L (ILoop ann (ArrowT τs1 τs2) es) (ArrowT τs1 τs2) L
-| TIte
-    (F : function_context) (L L' : local_context) (ann : A) (τa : arrow_type) (le : local_effect)
-    (es1 es2 : expr A) :
+  expr_has_type M F L es (ArrowT τs1 τs2) L ->
+  instr_has_type M F L (ILoop ann (ArrowT τs1 τs2) es) (ArrowT τs1 τs2) L
+| TIte M F L L' ann τa le es1 es2 :
   L' = update_locals le L ->
-  expr_has_type F L es1 τa L' ->
-  expr_has_type F L es2 τa L' ->
-  instr_has_type F L (IIte ann τa le es1 es2) τa L'
-| TBr
-    (F : function_context) (L L' : local_context) (ann : A) (n : nat) (τs τs1 τs2 : list type)
-    (le : local_effect) :
+  expr_has_type M F L es1 τa L' ->
+  expr_has_type M F L es2 τa L' ->
+  instr_has_type M F L (IIte ann τa le es1 es2) τa L'
+| TBr M F L L' ann n τs τs1 τs2 le :
   L' = update_locals le L ->
   F.(fc_labels) !! n = Some (τs, L) ->
   Forall (is_unrestricted F) τs1 ->
-  instr_has_type F L (IBr ann n) (ArrowT (τs1 ++ τs) τs2) L'
-| TBrIf (F : function_context) (L : local_context) (ann : A) (n : nat) (τs : list type) :
+  instr_has_type M F L (IBr ann n) (ArrowT (τs1 ++ τs) τs2) L'
+| TBrIf M F L ann n τs :
   F.(fc_labels) !! n = Some (τs, L) ->
-  instr_has_type F L (IBrIf ann n) (ArrowT (τs ++ [NumT (IntT I32T)]) τs) L
-| TBrTable
-    (F : function_context) (L L' : local_context) (ann : A) (ns : list nat) (n : nat)
-    (τs τs1 τs2 : list type) :
+  instr_has_type M F L (IBrIf ann n) (ArrowT (τs ++ [NumT (IntT I32T)]) τs) L
+| TBrTable M F L L' ann ns n τs τs1 τs2 :
   Forall (fun i => F.(fc_labels) !! i = Some (τs, L)) (n :: ns) ->
   Forall (is_unrestricted F) τs1 ->
-  instr_has_type F L (IBrTable ann ns n) (ArrowT (τs1 ++ τs ++ [NumT (IntT I32T)]) τs2) L'
-| TReturn
-    (F : function_context) (L L' : local_context) (ann : A) (le : local_effect)
-    (τs τs1 τs2 : list type) :
+  instr_has_type M F L (IBrTable ann ns n) (ArrowT (τs1 ++ τs ++ [NumT (IntT I32T)]) τs2) L'
+| TReturn M F L L' ann le τs τs1 τs2 :
   F.(fc_result_type) = τs ->
   L' = update_locals le L ->
   Forall (is_unrestricted F) τs1 ->
-  instr_has_type F L (IReturn ann) (ArrowT (τs1 ++ τs) τs2) L'
-| TLocalGet
-    (F : function_context) (L L' : local_context) (ann : A) (n : nat) (τ : type) (r : representation) :
+  instr_has_type M F L (IReturn ann) (ArrowT (τs1 ++ τs) τs2) L'
+| TLocalGet M F L L' ann n τ r :
   L !! n = Some τ ->
   has_rep F τ r ->
   L' = <[ n := RepT r (ProdT []) ]> L ->
-  instr_has_type F L (ILocalGet ann n) (ArrowT [] [τ]) L'
-| TLocalGetUnr (F : function_context) (L : local_context) (ann : A) (n : nat) (τ : type) :
+  instr_has_type M F L (ILocalGet ann n) (ArrowT [] [τ]) L'
+| TLocalGetUnr M F L ann n τ :
   L !! n = Some τ ->
   is_unrestricted F τ ->
-  instr_has_type F L (ILocalGet ann n) (ArrowT [] [τ]) L
-| TLocalSet
-    (F : function_context) (L L' : local_context) (ann : A) (n : nat) (τ τ' : type) (r : representation) :
+  instr_has_type M F L (ILocalGet ann n) (ArrowT [] [τ]) L
+| TLocalSet M F L L' ann n τ τ' r :
   L' = <[ n := τ' ]> L ->
   L !! n = Some τ ->
   is_unrestricted F τ ->
   has_rep F τ r ->
   has_rep F τ' r ->
-  instr_has_type F L (ILocalSet ann n) (ArrowT [τ'] []) L'
+  instr_has_type M F L (ILocalSet ann n) (ArrowT [τ'] []) L'
+| TGlobalGet M F L ann n m τ :
+  M.(mc_globals) !! n = Some (GlobalT m τ) ->
+  instr_has_type M F L (IGlobalGet ann n) (ArrowT [] [τ]) L
+| TGlobalSet M F L ann n m τ :
+  M.(mc_globals) !! n = Some (GlobalT m τ) ->
+  instr_has_type M F L (IGlobalSet ann n) (ArrowT [τ] []) L
 
 with expr_has_type {A : Type} :
-  function_context -> local_context -> expr A -> arrow_type -> local_context -> Prop :=
-| TNil (F : function_context) (L : local_context) :
-  expr_has_type F L [] (ArrowT [] []) L
-| TCons
-    (F : function_context) (L1 L2 L3 : local_context) (e : instr A) (es : expr A)
-    (τs1 τs2 τs3 : list type) :
-  instr_has_type F L1 e (ArrowT τs1 τs2) L2 ->
-  expr_has_type F L2 es (ArrowT τs2 τs3) L3 ->
-  expr_has_type F L1 (e :: es) (ArrowT τs1 τs3) L3.
+  module_ctx -> function_ctx -> local_ctx -> expr A -> arrow_type -> local_ctx -> Prop :=
+| TNil M F L :
+  expr_has_type M F L [] (ArrowT [] []) L
+| TCons M F L1 L2 L3 e es τs1 τs2 τs3 :
+  instr_has_type M F L1 e (ArrowT τs1 τs2) L2 ->
+  expr_has_type M F L2 es (ArrowT τs2 τs3) L3 ->
+  expr_has_type M F L1 (e :: es) (ArrowT τs1 τs3) L3.
